wf_table

proofs/compiler/stack_alloc_proof.v
@@ -199,6 +199,23 @@ Definition eq_vm (vm1 vm2:Vm.t) :=
     ~ Sv.In x pmap.(vnew) ->
     vm1.[x] = vm2.[x].
 
+(* Well-formedness of a [table] *)
+Definition wft_VARS table :=
+  forall x e,
+    Mvar.get table.(bindings) x = Some e ->
+    Sv.Subset (read_e e) table.(vars).
+
+Definition wft_SEM table se vm1 :=
+  forall x e v,
+    Mvar.get table.(bindings) x = Some e ->
+    get_var true vm1 x = ok v ->
+    sem_pexpr true [::] se e = ok v.
+
+Record wf_table table se vm1 := {
+  wft_vars : wft_VARS table;
+  wft_sem : wft_SEM table se vm1;
+}.
+
 (* Well-formedness of a [region]. *)
 Record wf_region (r : region) := {
   wfr_slot     : Sv.In r.(r_slot) Slots;
@@ -255,7 +272,7 @@ Record wf_sub_region se (sr : sub_region) ty := {
   wfsr_zone   :> wf_zone se sr.(sr_zone) ty sr.(sr_region).(r_slot)
 }.
 
-Definition wfr_WF se (rmap : region_map) :=
+Definition wfr_WF (rmap : region_map) se :=
   forall x sr,
     Mvar.get rmap.(var_region) x = Some sr ->
     wf_sub_region se sr x.(vtype).
@@ -304,7 +321,7 @@ Definition eq_sub_region_val_read se (m2:mem) sr status v :=
      get_val_byte v off = ok w ->
      read m2 Aligned (ofs + wrepr _ off)%R U8 = ok w.
 
-Definition eq_sub_region_val se ty m2 sr bytes v :=
+Definition eq_sub_region_val ty se m2 sr bytes v :=
   eq_sub_region_val_read se m2 sr bytes v /\
   (* According to the psem semantics, a variable of type [sword ws] can store
      a value of type [sword ws'] of shorter size (ws' <= ws).
@@ -349,12 +366,12 @@ Definition f rmap x :=
   get_gsub_region_status rmap x.(gv) vpk.
 *)
 
-Definition wfr_VAL se (rmap:region_map) (s1:estate) (s2:estate) :=
+Definition wfr_VAL (rmap:region_map) se (s1:estate) (s2:estate) :=
   forall x sr bytes v, check_gvalid rmap x = Some (sr, bytes) -> 
     get_gvar true gd s1.(evm) x = ok v ->
-    eq_sub_region_val se x.(gv).(vtype) s2.(emem) sr bytes v.
+    eq_sub_region_val x.(gv).(vtype) se s2.(emem) sr bytes v.
 
-Definition valid_pk se rmap (s2:estate) sr pk :=
+Definition valid_pk rmap se (s2:estate) sr pk :=
   match pk with
   | Pdirect s ofs ws cs sc =>
     sr = sub_region_direct s ws cs sc
@@ -369,14 +386,14 @@ Definition valid_pk se rmap (s2:estate) sr pk :=
     s2.(evm).[p] = Vword ofs
   end.
 
-Definition wfr_PTR se (rmap:region_map) (s2:estate) :=
+Definition wfr_PTR (rmap:region_map) se (s2:estate) :=
   forall x sr, Mvar.get (var_region rmap) x = Some sr ->
-    exists pk, get_local pmap x = Some pk /\ valid_pk se rmap s2 sr pk.
+    exists pk, get_local pmap x = Some pk /\ valid_pk rmap se s2 sr pk.
 
-Class wf_rmap se (rmap:region_map) (s1:estate) (s2:estate) := {
-  wfr_wf  : wfr_WF se rmap;
+Class wf_rmap (rmap:region_map) se (s1:estate) (s2:estate) := {
+  wfr_wf  : wfr_WF rmap se;
     (* sub-regions in [rmap] are well-formed *)
-  wfr_val : wfr_VAL se rmap s1 s2;
+  wfr_val : wfr_VAL rmap se s1 s2;
     (* [rmap] remembers for each relevant program variable which part of the target
        memory contains the value that this variable has in the source. These pieces
        of memory can be safely read without breaking semantics preservation.
@@ -385,7 +402,7 @@ Class wf_rmap se (rmap:region_map) (s1:estate) (s2:estate) := {
        the corresponding byte in the source. If a byte is not set, then there
        is no information.
     *)
-  wfr_ptr : wfr_PTR se rmap s2;
+  wfr_ptr : wfr_PTR rmap se s2;
     (* a variable in [rmap] is also in [pmap] and there is a link between
        the values associated to this variable in both maps *)
 }.
@@ -400,7 +417,7 @@ Hypothesis wf_pmap0 : wf_pmap.
    [s1]: current source estate
    [s2]: current target estate
 *)
-Class valid_state se (rmap : region_map) (m0 : mem) (s1 s2 : estate) := {
+Class valid_state table (rmap : region_map) se (m0 : mem) (s1 s2 : estate) := {
   vs_scs         : s1.(escs) = s2.(escs);
   vs_slot_valid  : slot_valid s2.(emem);
     (* slots are valid in the target *)
@@ -420,7 +437,8 @@ Class valid_state se (rmap : region_map) (m0 : mem) (s1 s2 : estate) := {
   vs_eq_vm       : eq_vm s1.(evm) s2.(evm);
     (* registers already present in the source program store the same values
        in the source and in the target *)
-  vs_wf_region   : wf_rmap se rmap s1 s2;
+  vs_wf_table    : wf_table table se s1.(evm);
+  vs_wf_region   : wf_rmap rmap se s1 s2;
     (* cf. [wf_rmap] definition *)
   vs_eq_mem      : eq_mem_source s1.(emem) s2.(emem);
     (* the memory that is already valid in the source is the same in the target *)
@@ -445,8 +463,8 @@ Proof.
   by split=> /=; lia.
 Qed.
 
-Lemma check_gvalid_wf se rmap x sr_bytes :
-  wfr_WF se rmap ->
+Lemma check_gvalid_wf rmap se x sr_bytes :
+  wfr_WF rmap se ->
   check_gvalid rmap x = Some sr_bytes ->
   wf_sub_region se sr_bytes.1 x.(gv).(vtype).
 Proof.
@@ -456,10 +474,10 @@ Proof.
   by case heq: Mvar.get => // -[<-]; apply hwfr.
 Qed.
 
-Definition valid_vpk se rv s2 x sr vpk :=
+Definition valid_vpk rv se s2 x sr vpk :=
   match vpk with
   | VKglob (_, ws) => sr = sub_region_glob x ws
-  | VKptr pk => valid_pk se rv s2 sr pk
+  | VKptr pk => valid_pk rv se s2 sr pk
   end.
 
 Lemma get_globalP x z : get_global pmap x = ok z <-> Mvar.get pmap.(globals) x = Some z.
@@ -469,11 +487,11 @@ Proof.
 Qed.
 
 (* A variant of [wfr_PTR] for [gvar]. *)
-Lemma wfr_gptr se rmap s1 s2 x sr bytes :
-  wf_rmap se rmap s1 s2 ->
+Lemma wfr_gptr rmap se s1 s2 x sr bytes :
+  wf_rmap rmap se s1 s2 ->
   check_gvalid rmap x = Some (sr, bytes) ->
   exists vpk, get_var_kind pmap x = ok (Some vpk)
-  /\ valid_vpk se rmap s2 x.(gv) sr vpk.
+  /\ valid_vpk rmap se s2 x.(gv) sr vpk.
 Proof.
   move=> hrmap.
   rewrite /check_gvalid /get_var_kind.
@@ -1089,8 +1107,8 @@ Qed.
 *)
 (* -------------------------------------------------------------------------- *)
 
-Lemma valid_incl_word se rmap m0 s1 s2 al p ws :
-  valid_state se rmap m0 s1 s2 ->
+Lemma valid_incl_word table rmap se m0 s1 s2 al p ws :
+  valid_state table rmap se m0 s1 s2 ->
   validw s1.(emem) al p ws ->
   validw s2.(emem) al p ws.
 Proof.
@@ -1101,8 +1119,8 @@ Proof.
   exact: hvalid.
 Qed.
 
-Lemma eq_mem_source_word se rmap m0 s1 s2 al p ws :
-  valid_state se rmap m0 s1 s2 ->
+Lemma eq_mem_source_word table rmap se m0 s1 s2 al p ws :
+  valid_state table rmap se m0 s1 s2 ->
   validw s1.(emem) al p ws ->
   read s1.(emem) al p ws = read s2.(emem) al p ws.
 Proof.
@@ -1197,8 +1215,9 @@ Proof.
 Qed.
 
 Section EXPR.
-  Variables (se : estate) (rmap:region_map) (m0:mem) (s:estate) (s':estate).
-  Hypothesis (hvalid: valid_state se rmap m0 s s').
+  Variables (table : table) (rmap:region_map).
+  Variables (se : estate) (m0:mem) (s:estate) (s':estate).
+  Hypothesis (hvalid: valid_state table rmap se m0 s s').
 
   (* If [x] is a register, it is not impacted by the presence of global
      variables per hypothesis [vs_eq_vm].
@@ -1394,7 +1413,7 @@ Section EXPR.
 *)
   Lemma addr_from_pkP wdb (x:var_i) pk sr ty xi ofs :
     wf_local x pk ->
-    valid_pk se rmap s' sr pk ->
+    valid_pk rmap se s' sr pk ->
     wf_sub_region se sr ty ->
     addr_from_pk pmap x pk = ok (xi, ofs) ->
     exists2 w,
@@ -1436,7 +1455,7 @@ Section EXPR.
 *)
   Lemma addr_from_vpkP wdb (x:var_i) vpk sr ty xi ofs :
     wf_vpk x vpk ->
-    valid_vpk se rmap s' x sr vpk ->
+    valid_vpk rmap se s' x sr vpk ->
     wf_sub_region se sr ty ->
     addr_from_vpk pmap x vpk = ok (xi, ofs) ->
     exists2 w,
@@ -1593,7 +1612,7 @@ Section EXPR.
       t_xrbindP=> hcvalid halign [xi ofsi] haddr [<-] hget /= htr.
       have hgvalid := get_gsub_region_statusP hgvk hgsub.
       have hwf := [elaborate check_gvalid_wf wfr_wf hgvalid].
-      have hvpk: valid_vpk se rmap s' x.(gv) sr vpk.
+      have hvpk: valid_vpk rmap se s' x.(gv) sr vpk.
       + have /wfr_gptr := hgvalid.
         by rewrite hgvk => -[_ [[]] <-].
       have [wi ok_wi eq_addr] :=
@@ -1632,7 +1651,7 @@ Section EXPR.
       t_xrbindP=> hcvalid halign [xi ofsi] haddr [<-] /=.
       have hgvalid := get_gsub_region_statusP hgvk hgsub.
       have hwf := [elaborate check_gvalid_wf wfr_wf hgvalid].
-      have hvpk: valid_vpk se rmap s' x.(gv) sr vpk.
+      have hvpk: valid_vpk rmap se s' x.(gv) sr vpk.
       + have /wfr_gptr := hgvalid.
         by rewrite hgvk => -[_ [[]] <-].
       have [wi ok_wi eq_addr] :=
@@ -1708,10 +1727,10 @@ Section EXPR.
 
 End EXPR.
 
-Lemma get_localn_checkg_diff se rmap sr_bytes s2 x y : 
+Lemma get_localn_checkg_diff rmap sr_status se s2 x y :
   get_local pmap x = None ->
-  wfr_PTR se rmap s2 ->
-  check_gvalid rmap y = Some sr_bytes ->
+  wfr_PTR rmap se s2 ->
+  check_gvalid rmap y = Some sr_status ->
   (~is_glob y -> x <> (gv y)).
 Proof.
   rewrite /check_gvalid; case:is_glob => // hl hwf.
@@ -1719,17 +1738,271 @@ Proof.
   by have /hwf [pk [hy _]] := heq; congruence.
 Qed.
 
-Lemma valid_state_set_var se rmap m0 s1 s2 x v:
-  valid_state se rmap m0 s1 s2 ->
+Variable (clone : (var_i → PrimInt63.int → var_i)).
+Context (clone_ty : forall x n, (clone x n).(vtype) = x.(vtype)).
+
+Notation symbolic_of_pexpr := (symbolic_of_pexpr clone).
+Notation get_symbolic_of_pexpr := (get_symbolic_of_pexpr clone).
+Notation update_table := (update_table clone).
+
+Section SYMBOLIC_OF_PEXPR_VARS.
+
+Let X e := forall table table' e',
+  symbolic_of_pexpr table e = Some (table', e') ->
+  wft_VARS table -> [/\
+    wft_VARS table',
+    Sv.Subset table.(vars) table'.(vars) &
+    Sv.Subset (read_e e') table'.(vars)].
+
+Let Y es := forall table table' es',
+  fmapo symbolic_of_pexpr table es = Some (table', es') ->
+  wft_VARS table -> [/\
+    wft_VARS table',
+    Sv.Subset table.(vars) table'.(vars) &
+    Sv.Subset (read_es es') table'.(vars)].
+
+Lemma symbolic_of_pexpr_vars_e_es :
+  (forall e, X e) /\ (forall es, Y es).
+Proof.
+  apply: pexprs_ind_pair; split; subst X Y => //=.
+  + move=> table _ _ [<- <-] hvars.
+    split=> //.
+    rewrite /read_es /=.
+    by clear; SvD.fsetdec.
+  + move=> e he es hes table table' es'.
+    apply: obindP => -[table1 e'] /he{}he.
+    apply: obindP => -[table2 {}es'] /= /hes{}hes [<- <-] hvars.
+    have [hvars1 hsub1 hsubr1] := he hvars.
+    have [hvars2 hsub2 hsubr2] := hes hvars1.
+    split=> //.
+    + by clear -hsub1 hsub2; SvD.fsetdec.
+    rewrite read_es_cons.
+    by clear -hsubr1 hsub2 hsubr2; SvD.fsetdec.
+  + move=> z table _ _ [<- <-] hvars.
+    split=> //.
+    rewrite /read_e /=.
+    by clear; SvD.fsetdec.
+  + move=> b table _ _ [<- <-] hvars.
+    split=> //.
+    rewrite /read_e /=.
+    by clear; SvD.fsetdec.
+  + move=> x table table' e'.
+    case: is_lvar => //.
+    rewrite /table_get_var.
+    case hget: Mvar.get => [e|].
+    + move=> [<- <-] hvars.
+      split=> //.
+      by apply: hvars hget.
+    rewrite /table_fresh_var /=.
+    case: Sv_memP => // hnin.
+    move=> [<- <-] hvars /=.
+    split.
+    + move=> y ey /=.
+      rewrite Mvar.setP.
+      case: eq_op.
+      + move=> [<-] /=.
+        rewrite read_e_var /read_gvar /=.
+        by clear; SvD.fsetdec.
+      move=> /hvars.
+      by clear; SvD.fsetdec.
+    + by clear; SvD.fsetdec.
+    rewrite read_e_var /read_gvar /=.
+    by clear; SvD.fsetdec.
+  + move=> op e he table table' e'.
+    apply: obindP => -[{}table' {}e'] /he{}he [<- <-] hvars.
+    have [hvars' hsub hsubr] := he hvars.
+    by split.
+  + move=> op e1 he1 e2 he2 table table' e'.
+    apply: obindP => -[table1 e1'] /he1{}he1.
+    apply: obindP => -[table2 e2'] /he2{}he2.
+    move=> [<- <-] hvars.
+    have [hvars1 hsub1 hsubr1] := he1 hvars.
+    have [hvars2 hsub2 hsubr2] := he2 hvars1.
+    split=> //.
+    + by clear -hsub1 hsub2; SvD.fsetdec.
+    rewrite read_e_Papp2.
+    by clear -hsubr1 hsub2 hsubr2; SvD.fsetdec.
+  + move=> op es hes table table' e'.
+    apply: obindP => -[table1 es'] /hes{}hes.
+    move=> [<- <-] hvars.
+    have [hvars1 hsub1 hsubr1] := hes hvars.
+    by split.
+  move=> ty b hb e1 he1 e2 he2 table table' e'.
+  apply: obindP => -[table1 b'] /hb{}hb.
+  apply: obindP => -[table2 e1'] /he1{}he1.
+  apply: obindP => -[table3 e2'] /he2{}he2.
+  move=> [<- <-] hvars.
+  have [hvars1 hsub1 hsubr1] := hb hvars.
+  have [hvars2 hsub2 hsubr2] := he1 hvars1.
+  have [hvars3 hsub3 hsubr3] := he2 hvars2.
+  split=> //.
+  + by clear -hsub1 hsub2 hsub3; SvD.fsetdec.
+  rewrite read_e_Pif.
+  by clear -hsubr1 hsub2 hsubr2 hsub3 hsubr3; SvD.fsetdec.
+Qed.
+
+Lemma wft_VARS_symbolic_of_pexpr table table' e e' :
+  symbolic_of_pexpr table e = Some (table', e') ->
+  wft_VARS table ->
+  wft_VARS table'.
+Proof.
+  move=> he hvars.
+  by have [hvars' _ _] := symbolic_of_pexpr_vars_e_es.1 _ _ _ _ he hvars.
+Qed.
+
+(* Actually, the hypothesis wft_VARS is not needed, but is was simpler to prove
+   the 3 propositions in one go. *)
+Lemma symbolic_of_pexpr_subset_vars table table' e e' :
+  symbolic_of_pexpr table e = Some (table', e') ->
+  wft_VARS table ->
+  Sv.Subset table.(vars) table'.(vars).
+Proof.
+  move=> he hvars.
+  by have [_ hsub _] := symbolic_of_pexpr_vars_e_es.1 _ _ _ _ he hvars.
+Qed.
+
+Lemma symbolic_of_pexpr_subset_read table table' e e' :
+  symbolic_of_pexpr table e = Some (table', e') ->
+  wft_VARS table ->
+  Sv.Subset (read_e e') table'.(vars).
+Proof.
+  move=> he hvars.
+  by have [_ _ hsubr] := symbolic_of_pexpr_vars_e_es.1 _ _ _ _ he hvars.
+Qed.
+
+End SYMBOLIC_OF_PEXPR_VARS.
+
+Section SYMBOLIC_OF_PEXPR_SEM.
+
+Context (vm : Vm.t).
+
+Let X e := forall table table' e' se,
+  symbolic_of_pexpr table e = Some (table', e') ->
+  wf_table table se vm ->
+  exists se',
+    wft_SEM table' se' vm.
+
+Let Y es := forall table table' es' se,
+  fmapo symbolic_of_pexpr table es = Some (table', es') ->
+  wf_table table se vm ->
+  exists se',
+    wft_SEM table' se' vm.
+
+Lemma tes : (forall e, X e) /\ (forall es, Y es).
+Proof.
+  apply: pexprs_ind_pair; split; subst X Y => //=.
+  - move=> table _ _ se [<- _] [_ hsem].
+    by exists se.
+  - move=> e he es hes table table' es' se.
+    apply: obindP => -[table1 e'] /[dup] H /he{}he.
+    apply: obindP => -[table2 {}es'] /= /hes{}hes [<- _] hsem.
+    have [se1 hsem1] := he _ hsem.
+    have := wft_VARS_symbolic_of_pexpr H hsem.(wft_vars).
+    have [se2 hsem2] := hes _ hsem1.
+    by exists se2.
+  - move=> _ table _ _ se [<- _] hsem.
+    by exists se.
+  - move=> _ table _ _ se [<- _] hsem.
+    by exists se.
+  - move=> x table table' e' se.
+    case: is_lvar => //.
+    rewrite /table_get_var.
+    case hget: Mvar.get => [e|].
+    + move=> [<- _] hsem.
+      by exists se.
+    rewrite /table_fresh_var.
+    case: Sv_memP => // ?.
+    move=> [<- _] hsem.
+    set x' := clone x.(gv) _.
+    exists (with_vm se se.(evm).[x' <- vm.[x.(gv)]]).
+    move=> y ey vy /=.
+    rewrite Mvar.setP.
+    case: eqP.
+    + move=> ? [<-] /=.
+      rewrite /get_gvar /= /get_var Vm.setP_eq.
+      rewrite compat_val_vm_truncate_val. subst y. done.
+      rewrite clone_ty. apply Vm.getP.
+    move=> ? /[dup] h /hsem{}hsem /hsem <-.
+    apply eq_on_sem_pexpr. done.
+    simpl.
+    move=> ??. rewrite Vm.setP_neq. done. apply /eqP.
+     have H: wft_VARS table. admit. have := H _ _ h.
+     move=> op hj.
+     match goal with | [ k : ~ Sv.In _ _ |- _] => case: k end.
+     apply op. rewrite /x' in hj. congruence.
+  - move=> op e he table table' e' se.
+    apply: obindP => -[{}table' {}e'] /he{}he [<- _] hsem.
+    have [se1 hsem1] := he _ hsem.
+    by exists se1.
+  - move=> op e1 he1 e2 he2 table table' e' se.
+    apply: obindP => -[table1 e1'] /he1{}he1.
+    apply: obindP => -[table2 e2'] /he2{}he2.
+    move=> [<- _] hsem.
+    have [se1 hsem1] := he1 _ hsem.
+    have [se2 hsem2] := he2 _ hsem1.
+    by exists se2.
+  + move=> op es hes table table' e' se.
+    apply: obindP => -[table1 es'] /hes{}hes.
+    move=> [<- _] hsem.
+    have [se1 hsem1] := hes _ hsem.
+    by exists se1.
+  move=> ty b hb e1 he1 e2 he2 table table' e' se.
+  apply: obindP => -[table1 b'] /hb{}hb.
+  apply: obindP => -[table2 e1'] /he1{}he1.
+  apply: obindP => -[table3 e2'] /he2{}he2.
+  move=> [<- _] hsem.
+  have [se1 hsem1] := hb _ hsem.
+  have [se2 hsem2] := he1 _ hsem1.
+  have [se3 hsem3] := he2 _ hsem2.
+  by exists se3.
+Qed.
+
+Lemma wf_table_set_var table se s1 e v r s1' :
+  wf_table table se (evm s1) ->
+  sem_pexpr true gd s1 e = ok v ->
+  write_lval true gd r v s1 = ok s1' ->
+  exists se',
+    wf_table (update_table table r e) se' (evm s1').
+Proof.
+  case: r => /=.
+  + move=> _ ? hwf _ /write_noneP [-> _ _]. exists se. done.
+  + move=> x hwf hsem hw.
+    case h: symbolic_of_pexpr => [[table' e']|].
+    + exists (with_vm se (evm se).[x <- v]).
+      split.
+      + have H := wft_VARS_symbolic_of_pexpr h hwf.(wft_vars).
+        move=> y ey /=.
+        rewrite Mvar.setP.
+        case: eqP.
+        + move=> _ [<-]. apply (symbolic_of_pexpr_subset_read h). apply hwf.(wft_vars).
+        move=> _. apply H.
+      move=> ? /= ??.
+      rewrite Mvar.setP.
+      case: eqP.
+      + move=> <- [<-] /=. move=> ?. admit.
+      move=> _ hget okv.
+      have := hwf.(wft_sem) hget.
+  + t_xrbindP=> ???? hwf _ ?? _ _ ?? _ _ ? _ ? _ <- /=.
+    exists se. done.
+  (* invariant: table ne contient que des sword ? *)
+
+Lemma valid_state_set_var table rmap se m0 s1 s2 x v:
+  valid_state table rmap se m0 s1 s2 ->
   get_local pmap x = None ->
   ¬ Sv.In x (vnew pmap) ->
-  valid_state se rmap m0 (with_vm s1 (evm s1).[x <- v]) (with_vm s2 (evm s2).[x <- v]).
+  valid_state table rmap se m0 (with_vm s1 (evm s1).[x <- v]) (with_vm s2 (evm s2).[x <- v]).
 Proof.
-  case: s1 s2 => scs1 mem1 vm1 [scs2 mem2 vm2] [/=] hscs hvalid hdisj hincl hincl2 hunch hrip hrsp heqvm hwfr heqmem hglobv htop hget hnin.
+  case: s1 s2 => scs1 mem1 vm1 [scs2 mem2 vm2].
+  case=>
+    /= hscs hvalid hdisj hincl hincl2 hunch hrip hrsp heqvm hwft hwfr heqmem
+    hglobv htop hget hnin.
   constructor => //=.
   + by rewrite Vm.setP_neq //; assert (h:=rip_in_new); apply/eqP => ?; subst x; apply hnin.
   + by rewrite Vm.setP_neq //; assert (h:=rsp_in_new); apply/eqP => ?; subst x; apply hnin.
   + by move=> y hy hnnew; rewrite !Vm.setP heqvm.
+  + case: hwft => hvars hsem.
+    constructor=> //.
+    
   rewrite /with_vm /=; case: hwfr => hwfsr hval hptr.
   constructor => //.
   + move=> y sr bytes vy hy; have ? := get_localn_checkg_diff hget hptr hy.
